More lemmas to verify backtranslation

rupicola/io/Backtranslation.fst
@@ -143,6 +143,56 @@ let rec backtranslate' #g #e #t h : Tot (fs_oprod g t) =
     let h3 : typing (extend t2 g) _ t3 = h3 in
     fs_oprod_case (backtranslate' h1) (backtranslate' h2) (backtranslate' h3)
 
+let rec lem_backtranslate' #g #e #t (h:typing g e t) : Lemma (backtranslate' h ≋ e)=
+   match e with
+  | EUnit -> equiv_oprod_unit g
+  | ETrue -> equiv_oprod_true g
+  | EFalse -> equiv_oprod_false g
+  | EIf _ _ _ ->
+    let TyIf #_ #e1 #e2 #e3 h1 h2 h3 = h in
+    lem_backtranslate' h1;
+    lem_backtranslate' h2;
+    lem_backtranslate' h3;
+    equiv_oprod_if (backtranslate' h1) (backtranslate' h2) (backtranslate' h3) e1 e2 e3
+  | EFileDescr fd -> equiv_oprod_file_descr g fd
+  | EVar x -> equiv_oprod_var g x
+  | EApp _ _ ->
+    let TyApp #t1 #t2 #e1 #e2 h1 h2 = h in
+    lem_backtranslate' h1;
+    lem_backtranslate' h2;
+    equiv_oprod_app (backtranslate' h1) (backtranslate' h2) e1 e2
+  | ELam _ ->
+    let TyLam #t1 #t2 #body hbody = h in
+    lem_backtranslate' hbody;
+    equiv_oprod_lambda (backtranslate' hbody) body
+  | EPair _ _ ->
+    let TyPair #_ #e1 #e2 #t1 #t2 h1 h2 = h in
+    lem_backtranslate' h1;
+    lem_backtranslate' h2;
+    equiv_oprod_pair (backtranslate' h1) (backtranslate' h2) e1 e2
+  | EFst _ ->
+    let TyFst #t1 #t2 #e' h' = h in
+    lem_backtranslate' h';
+    equiv_oprod_fst (backtranslate' h') e'
+  | ESnd _ ->
+    let TySnd #t2 #t1 #e' h' = h in
+    lem_backtranslate' h';
+    equiv_oprod_snd (backtranslate' h') e'
+  | EInl _ ->
+    let TyInl #t1 t2 #e' h' = h in
+    lem_backtranslate' h';
+    equiv_oprod_inl t1 t2 (backtranslate' h') e'
+  | EInr _ ->
+    let TyInr t1 #t2 #e' h' = h in
+    lem_backtranslate' h';
+    equiv_oprod_inr t1 t2 (backtranslate' h') e'
+  | ECase _ _ _ ->
+    let TyCase #t1 #t2 #t3 #e1 #e2 #e3 h1 h2 h3 = h in
+    lem_backtranslate' h1;
+    lem_backtranslate' h2;
+    lem_backtranslate' h3;
+    equiv_oprod_case (backtranslate' h1) (backtranslate' h2) (backtranslate' h3) e1 e2 e3
+
 let rec lem_backtranslate_value_no_io (#g:typ_env) (#e:value) (#t:qType) (h:typing g e t) (fsG:eval_env g) :
   Pure (fs_val t) True (fun v -> return v == backtranslate' h fsG) =
   let r = backtranslate' h fsG in
@@ -176,108 +226,3 @@ let rec lem_backtranslate_value_no_io (#g:typ_env) (#e:value) (#t:qType) (h:typi
   | EFst _
   | ESnd _
   | ECase _ _ _ -> assert False
-
-let equiv_val_are_equiv_prods (#g:typ_env) (#t:qType) (fs_v:fs_oval g t) (e:exp) :
-  Lemma
-    (requires (fs_v ≈ e))
-    (ensures (helper_return_prod fs_v ≋ e))
-  [SMTPat (fs_v ≈ e)] =
-  equiv_oprod_return fs_v e
-
-
-let rec lem_backtranslate' #g #e #t (h:typing g e t) : Lemma (backtranslate' h ≋ e)=
-   match e with
-  | EUnit ->
-    equiv_unit g;
-    let r = lem_backtranslate_value_no_io h in
-    equiv_oprod_return r e
-  | EVar x ->
-    equiv_var g x;
-    equiv_oprod_return #g #_ (fun (fsG:eval_env g) -> index fsG x) e
-  | EApp e1 e2 ->
-    let TyApp #t1 #t2 #_ #_ #g h1 h2 = h in
-    assert (t == t2);
-    lem_fv_in_env_app g e1 e2;
-    let fs_e1 : fs_oprod g (t1 ^->!@ t2) = backtranslate' h1 in
-    lem_backtranslate' h1;
-    assert (fs_e1 ≋ e1);
-    let fs_e2 : fs_oprod g t1 = backtranslate' h2 in
-    lem_backtranslate' h2;
-    assert (fs_e2 ≋ e2);
-//    let fs_e = (fun fsG ->
-//      let!@ f' = fs_e1 fsG in
-//      let!@ x' = fs_e2 fsG in
-//      f' x') in
- //   equiv_oprod_bind #_ #t1 #t2 fs_e2 fs_e1 e2 e1;
-    equiv_oprod_app' fs_e1 fs_e2 e1 e2;
-    assert (backtranslate' h == (fun fsG ->
-      let!@ f' = fs_e1 fsG in
-      let!@ x' = fs_e2 fsG in
-      f' x')) by (
-        rewrite_eqs_from_context ();
-        norm [delta_once [`%backtranslate'];iota];
-        tadmit ())
-  | _ -> admit ()
-
-let _ = ()
-(**
-  | ELam _ ->
-    let TyLam #t1 #t2 #body hbody = h in
-    lem_fv_in_env_lam g t1 body;
-    lem_backtranslate' hbody;
-    equiv_lam_prod (backtranslate' hbody) body
-  | ETrue -> equiv_true g
-  | EFalse -> equiv_false g
-  | EIf e1 e2 e3 ->
-    let TyIf h1 h2 h3 = h in
-    lem_fv_in_env_if g e1 e2 e3;
-    lem_backtranslate' h1;
-    lem_backtranslate' h2;
-    lem_backtranslate' h3;
-    let fs_e1 = (backtranslate' h1) in
-    let fs_e2 = (backtranslate' h2) in
-    let fs_e3 = (backtranslate' h3) in
-    equiv_oprod_if fs_e1 fs_e2 fs_e3 e1 e2 e3
-  | EPair e1 e2 ->
-    let TyPair #_ #_ #_ #t1 #t2 h1 h2 = h in
-    lem_fv_in_env_pair g e1 e2;
-    lem_backtranslate' h1;
-    lem_backtranslate' h2;
-    let fs_e1 = (backtranslate' h1) in
-    let fs_e2 = (backtranslate' h2) in
-    equiv_pair #_ #t1 #t2 fs_e1 fs_e2 e1 e2
-  | EFst e12 ->
-    let TyFst #t1 #t2 h1 = h in
-    lem_fv_in_env_fst g e12;
-    lem_backtranslate' h1;
-    let fs_e12 = (backtranslate' h1) in
-    equiv_pair_fst_app #_ #t1 #t2 fs_e12 e12
-  | ESnd e12 ->
-    let TySnd #t1 #t2 h1 = h in
-    lem_fv_in_env_snd g e12;
-    lem_backtranslate' h1;
-    let fs_e12 = (backtranslate' h1) in
-    equiv_pair_snd_app #_ #t1 #t2 fs_e12 e12
-  | EInl e' ->
-    let TyInl #t1 t2 h' = h in
-    lem_fv_in_env_inl g e';
-    lem_backtranslate' h';
-    let fs_e' = backtranslate' h' in
-    equiv_inl #_ #t1 t2 fs_e' e'
-  | EInr e' ->
-    let TyInr t1 #t2 h' = h in
-    lem_fv_in_env_inr g e';
-    lem_backtranslate' h';
-    let fs_e' = backtranslate' h' in
-    equiv_inr t1 #t2 fs_e' e'
-  | ECase cond inlc inrc ->
-    let TyCase #t1 #t2 #t3 hcond hinlc hinrc = h in
-    lem_fv_in_env_case g t1 t2 cond inlc inrc;
-    lem_backtranslate' hcond;
-    lem_backtranslate' hinlc;
-    lem_backtranslate' hinrc;
-    let fs_cond = backtranslate' hcond in
-    let fs_inlc = backtranslate' hinlc in
-    let fs_inrc = backtranslate' hinrc in
-    equiv_oprod_case #_ #t1 #t2 #t3 fs_cond fs_inlc fs_inrc cond inlc inrc
- **)
